veric/SequentialClight.v
@@ -1,7 +1,7 @@
 Require Import VST.sepcomp.semantics.
 
 Require Import VST.veric.Clight_base.
-Require Import VST.veric.Clight_new.
+Require Import VST.veric.Clight_core.
 Require Import VST.veric.Clight_lemmas.
 Require Import VST.sepcomp.step_lemmas.
 Require Import VST.sepcomp.event_semantics.
@@ -9,7 +9,7 @@ Require Import VST.veric.SeparationLogic.
 Require Import VST.veric.juicy_extspec.
 Require Import VST.veric.juicy_mem.
 Require VST.veric.NullExtension.
-Require Import VST.veric.Clight_sim.
+(*Require Import VST.veric.Clight_sim.*)
 Require Import VST.veric.SeparationLogicSoundness.
 Require Import VST.sepcomp.extspec.
 Require Import VST.msl.msl_standard.
