veric/semax_conj_disj.v
@@ -4,7 +4,7 @@ Require Import VST.VST.veric.res_predicates.
 Require Import VST.veric.extend_tc.
 Require Import VST.veric.Clight_seplog.
 Require Import VST.veric.Clight_assert_lemmas.
-Require Import VST.veric.Clight_new.
+Require Import VST.veric.Clight_core.
 Require Import VST.sepcomp.extspec.
 Require Import VST.sepcomp.step_lemmas.
 Require Import VST.veric.tycontext.
