Makefile
@@ -236,13 +236,13 @@ VERIC_FILES= \
   binop_lemmas.v binop_lemmas2.v binop_lemmas3.v binop_lemmas4.v binop_lemmas5.v binop_lemmas6.v \
   expr_lemmas.v expr_lemmas2.v expr_lemmas3.v expr_lemmas4.v \
   extend_tc.v \
-  Clight_lemmas.v Clight_new.v Clightnew_coop.v Clight_core.v Clight_sim.v \
+  Clight_lemmas.v Clight_new.v Clightnew_coop.v Clight_core.v  \
   slice.v res_predicates.v own.v seplog.v Clight_seplog.v mapsto_memory_block.v Clight_mapsto_memory_block.v assert_lemmas.v Clight_assert_lemmas.v \
   juicy_mem.v juicy_mem_lemmas.v local.v juicy_mem_ops.v juicy_safety.v juicy_extspec.v \
   semax.v semax_lemmas.v semax_conseq.v semax_call.v semax_straight.v semax_loop.v semax_switch.v \
   initial_world.v Clight_initial_world.v initialize.v semax_prog.v semax_ext.v SeparationLogic.v SeparationLogicSoundness.v  \
   NullExtension.v SequentialClight.v superprecise.v jstep.v address_conflict.v valid_pointer.v coqlib4.v \
-  semax_ext_oracle.v mem_lessdef.v Clight_mem_lessdef.v Clight_sim.v age_to_resource_at.v aging_lemmas.v Clight_aging_lemmas.v ghost_PCM.v mpred.v
+  semax_ext_oracle.v mem_lessdef.v Clight_mem_lessdef.v age_to_resource_at.v aging_lemmas.v Clight_aging_lemmas.v ghost_PCM.v mpred.v
 
 FLOYD_FILES= \
    coqlib3.v base.v seplog_tactics.v typecheck_lemmas.v val_lemmas.v assert_lemmas.v find_nth_tactic.v const_only_eval.v \
